examples/List_Reversal.thy
@@ -1,6 +1,11 @@
 theory List_Reversal
   imports "ITree_UTP.ITree_UTP"
-begin lit_vars
+begin 
+
+term "[\<lambda> s. R i s]\<^sub>e"
+term "[\<lambda> s. R s i]\<^sub>e"
+
+lit_vars
 
 syntax
   "_kleisli_comp" :: "logic \<Rightarrow> logic \<Rightarrow> logic" (infixr ";" 54)
@@ -21,13 +26,17 @@ procedure reverse "xs :: int list" over state =
 
 procedure reverse' "xs :: int list" over state =
 "ys := [];
- for j in [0..<length xs] do ys := xs!j # ys od"
+ for x in xs inv j. ys = rev (take j xs) do ys := x # ys od"
 
 execute "reverse [1,2,3,4]"
 execute "reverse' [1,2,3,4]"
 
 lemma reverse_correct: "H{True} reverse xs {ys = rev xs}"
   unfolding reverse_def
+  by (hoare_auto, simp add: take_Suc_conv_app_nth)
+
+lemma reverse_correct': "H{True} reverse' xs {ys = rev xs}"
+  unfolding reverse'_def
   by (hoare_auto, simp add: take_Suc_conv_app_nth)
 
 end
